# AERE 310 HW 1

Abhigyaan Deep

## 1.

Given:

$$
f(x,y) = xy
$$

## 1. (a)

$$
f(x,y) = c = xy
$$

$$
y = \frac{c}{x}
$$

I chose all integers in $[-3, 3]$ to generate [the following Desmos level surfaces](https://www.desmos.com/calculator/yg04m60tc2):

![Level Surfaces](https://i.imgur.com/LiMsHTxl.png)

## 1. (b)

$$
\nabla f(x,y) = \langle \frac{\partial}{\partial x} xy, \frac{\partial}{\partial y} xy \rangle = \langle y, x \rangle
$$

I chose an $11 \times 11$ grid of points to generate [the following Desmos gradient vectors](https://www.desmos.com/calculator/p4rdywqtus):

![Gradient Vectors](https://i.imgur.com/2pMbB2kl.png)

[A GeoGebra applet](https://www.geogebra.org/m/QPE4PaDZ) also conveys the arrows:

![Gradient Vectors](https://i.imgur.com/VaIyaGbl.png)

## 2.

Given:

$$
\vec{V} = u \hat{i} = V_0 (1 - e^{-ct}) (1 - \frac{x}{l}) \hat{i}
$$

![Diffuser](https://i.imgur.com/RdS7XTRm.png)

## 2. (a)

We have already been given the velocity as a function of $x$ and $t$:

$$
\vec{V}(x,t) = V_0 (1 - e^{-ct}) (1 - \frac{x}{l}) \hat{i}
$$

Therefore, the acceleration can be derived directly:

$$
\vec{A}(x,t) = \frac{\partial \vec{V}}{\partial t}
$$

$$
\vec{A}(x,t) = V_0 \hat{i} \left[ \frac{\partial}{\partial t} \left((1-e^{-ct}) (1-\frac{x}{l}) \right) \right]
$$

$$
\vec{A}(x,t) = V_0 \hat{i} \left[ c e^{-ct} (1-\frac{x}{l}) + 0 \right]
$$

$$
\vec{A}(x,t) = \boxed{c V_0 e^{-ct} (1 - \frac{x}{l}) \hat{i}}
$$

# 2. (b)

$$
V_0=10ft/s
$$

$$
l=5ft
$$

$$
l=1s
$$

$$
c=0.49s^{-1}
$$

Here, $x=l$ since we are trying to find the "end" behavior by the end of the diffuser.

$$
\vec{A} = 0.49s^{-1} \times 10ft/s \times e^{-0.49s^{-1} \times 1s} (1 - \frac{5ft}{5ft}) \hat{i} = 0
$$

The $0$ originates from the fact that $x=l$. Thus, we end up dividing $l/l=1$. The equation then subtracts $1$ from $1$ to get $0$. Regardless of the values of other members of the product, the function returns $0$.

Intuitively, this behavior shouldn't be too otherworldly. An acceleration of $0$ does not imply a velocity of $0$. Sure, the liquid has stopped moving faster/slower, but it's still moving regardless. In other words, the diffuser has indeed diffused the liquid. Also the liquid is now starting to accelerate purely in the $\hat{j}$ direction.

## 3.

Given:

$$
u = \frac{cx}{x^2+y^2}
$$

$$
v = \frac{cy}{x^2+y^2}
$$

## 3. (a)

$$
V = \langle u, v \rangle
$$

$$
\frac{\Delta \delta V}{\Delta t} = \nabla \cdot V = \frac{\partial}{\partial x} \frac{cx}{x^2+y^2} + \frac{\partial}{\partial y} \frac{cy}{x^2+y^2}
$$

$$
\frac{\Delta \delta V}{\Delta t} = \frac{c (y^2 - x^2)}{(x^2 + y^2)^2} + \frac{c (x^2 - y^2)}{(x^2 + y^2)^2} = \frac{c (y^2 - x^2) + c (x^2 - y^2)}{(x^2 + y^2)^2} = \frac{c (y^2 - x^2 + x^2 - y^2)}{(x^2 + y^2)^2} = \boxed{0}
$$

$0$ makes sense as this is incompressible flow after all.

## 3. (b)

$$
w = \nabla \times V = \frac{\partial}{\partial x} v - \frac{\partial}{\partial y} u
$$

$$
w = \frac{\partial}{\partial x} \frac{cy}{x^2+y^2} - \frac{\partial}{\partial y} \frac{cx}{x^2+y^2}
$$

$$
w = \frac{-2cxy}{(x^2 + y^2)^2} - \frac{-2cxy}{(x^2 + y^2)^2} = \boxed{0}
$$

Once again, $0$ makes intuitive sense as the diffusor doesn't seem to have any geometry that could cause the liquid to "turn on itself" and moving retrograde to all other fluid particles.

## 4.

Given:

$$
d_p=55ft=16.76m
$$

$$
D_p=950lbf=4226N
$$

$$
u_p=12mi/h=5.364m/s
$$

$$
T_p=20\degree C=293.2K
$$

$$
p_p=1atm=101325Pa
$$

$$
d_m=1.7m
$$

$$
\rho=1kg/m^3
$$

$$
\mu=2*10^{-5}Pa*s
$$

## 4. (a)

$$
Re_m=Re_p
$$

$$
\frac{\rho u_m d_m}{\mu} = \frac{\rho u_p d_p}{\mu}
$$

$$
u_m = \frac{\cancel{\rho} u_p d_p \cancel{\mu}}{\cancel{\mu} \cancel{\rho} d_m} = \frac{u_p d_p}{d_m} = \frac{5.364m/s * 16.76m}{1.7m} = \boxed{52.9m/s}
$$

## 4. (b)

$$
\frac{1}{2} \rho u_p^2 C_D A_p = \frac{1}{2} \rho u_m^2 C_D A_m
$$

$$
\frac{D_p}{D_m} = 1 = \frac{\cancel{\frac{1}{2}} \cancel{\rho} u_p^2 \cancel{C_D} A_p}{\cancel{\frac{1}{2}} \cancel{\rho} u_m^2 \cancel{C_D} A_m} = \frac{u_p^2 A_p}{u_m^2 A_m}
$$

$$
D_m = \frac{D_p u_m^2 A_m}{u_p^2 A_p} = \frac{D_p u_m^2 \cancel{\frac{\pi}{4}} d_m^2}{u_p^2 \cancel{\frac{\pi}{4}} d_p^2} = \frac{D_p u_m^2 d_m^2}{u_p^2 d_p^2}
$$

$$
D_m = \frac{4226N * (52.9m/s)^2 * (1.7m)^2}{(5.364m/s)^2 * (16.76m)^2} = \boxed{4230N}
$$

## 4. (c)

$D_m$ is suspiciously to $D_p$ and I suspect this is due to some secret cancellations within the fraction of which the details I cannot see.
