# AERE 310 HW 2

Abhigyaan Deep

## 1.

$$
u=6xy
$$

$$
v=2x-3y^2
$$

## 1. (a)

$$
\frac{\partial u}{\partial x} + \frac{\partial v}{\partial y} = 0
$$

$$
\boxed{\cancel{6y} + \cancel{(-6y)} = 0}
$$

$$
u = \frac{\partial \psi}{\partial y}
$$

$$
\partial \psi = u \partial y = 6xy \partial y
$$

$$
\psi = 3xy^2 + f(x)
$$

$$
v = -\frac{\partial \psi}{\partial x} = -\frac{\partial (3xy^2 + f(x))}{\partial x}
$$

$$
v = \cancel{3y^2} + f'(x) = 2x - \cancel{3y^3}
$$

$$
f'(x) = 2x
$$

$$
f(x) = x^2 + c
$$

$$
\boxed{\psi = 3xy^2 + x^2 + c}
$$

## 1. (b)

The following Desmos stream lines use $c=0$ and $\Phi = \{ x \in \mathbb{Z} \mid -5 \leq x \leq 5 \}$ (all integers from $-5$ to $5$):

![](https://i.imgur.com/hXr9Gz8l.png)

https://www.desmos.com/calculator/zh0tdclq5f

## 2.

$$
v_r = 2r + 3r^2 \sin \theta
$$

$$
\frac{1}{r} \frac{\partial (r v_r)}{\partial r} + \frac{1}{r} \frac{\partial v_\theta}{\partial \theta} = 0
$$

$$
\frac{1}{r} \frac{\partial (r (2r + 3r^2 \sin \theta))}{\partial r} + \frac{1}{r} \frac{\partial v_\theta}{\partial \theta} = 0
$$

$$
\frac{1}{r} \frac{\partial (2r^2 + 3r^3 \sin \theta)}{\partial r} + \frac{1}{r} \frac{\partial v_\theta}{\partial \theta} = 0
$$

$$
\frac{1}{r} (4r + 9r^2 \sin \theta) + \frac{1}{r} \frac{\partial v_\theta}{\partial \theta} = 0
$$

$$
4 + 9r \sin \theta + \frac{1}{r} \frac{\partial v_\theta}{\partial \theta} = 0
$$

$$
\frac{1}{r} \frac{\partial v_\theta}{\partial \theta} = - =4 - 9r \sin \theta
$$

$$
\frac{\partial v_\theta}{\partial \theta} = -4r - 9r^2 \sin \theta
$$

$$
\partial v_\theta = (-4r - 9r^2 \sin \theta) \partial \theta
$$

$$
v_\theta = -4r\theta + 9r^2 \sin \theta + f(r)
$$

$$
\boxed{v_\theta = 9r^2 \sin \theta - 4r\theta + f(r)}
$$

## 3.

$$
u = x^2 - y^2 + x
$$

$$
v = -(2xy + y) = -2xy - y
$$

## 3. (a)

$$
\omega = \frac{\partial v}{\partial x} - \frac{\partial u}{\partial y} = 0
$$

$$
\frac{\partial (-2xy - y)}{\partial x} - \frac{\partial (x^2 - y^2 + x)}{\partial y} = 0
$$

$$
\boxed{\cancel{-2y} - \cancel{(-2y)} = 0}
$$

$$
u = \frac{\partial \phi}{\partial x}
$$

$$
\partial \phi = u \partial x = (x^2 - y^2 + x) \partial x
$$

$$
\phi = \frac{1}{3}x^3 - xy^2 + \frac{1}{2}x^2 + f(y)
$$

$$
v = \frac{\partial \phi}{\partial y} = \frac{\partial (\frac{1}{3}x^3 - xy^2 + \frac{1}{2}x^2 + f(y))}{\partial y}
$$

$$
v = \cancel{-2xy} + f'(y) = \cancel{-2xy} - y
$$

$$
f'(y) = -y
$$

$$
f(y) = -\frac{1}{2} y^2 + c
$$

$$
\boxed{\phi = \frac{1}{3}x^3 - xy^2 + \frac{1}{2}x^2 - \frac{1}{2} y^2 + c}
$$

## 3. (b)

$$
V = \langle u, v \rangle = \langle x^2 - y^2 + x, -2xy - y \rangle
$$

$$
P_0 = (0, 0)
$$

$$
P_1 = (2, 3)
$$

$$
t_0 = 0
$$

$$
t_1 = 1
$$

$$
x(t) = 2t
$$

$$
dx(t) = 2
$$

$$
y(t) = 3t
$$

$$
dy(t) = 3
$$

$$
d\vec{s} = \langle 2, 3 \rangle dt
$$

$$
V(t) = \langle (2t)^2 - (3t)^2 + 2t, -2(2t)(3t) - 3t \rangle
$$

$$
V(t) = \langle 4t^2 - 9t^2 + 2t, -12t^2 - 3t \rangle
$$

$$
V(t) = \langle -5t^2 + 2t, -12t^2 - 3t \rangle
$$

$$
\int_{(0, 0)}^{(2, 3)} V \cdot d\vec{s} = \int_0^1 V(t) \cdot \langle 2, 3 \rangle dt
$$

$$
\int_0^1 2(-5t^2 + 2t) + 3(-12t^2 - 3t) ~ dt
$$

$$
\int_0^1 -10t^2 + 4t + -36t^2 - 9t ~ dt
$$

$$
\int_0^1 -46t^2 - 5t ~ dt
$$

$$
\left[ -\frac{46}{3}t^3 - \frac{5}{2}t^2 \right]_0^1 = -\frac{46}{3} - \frac{5}{2} = \boxed{-\frac{107}{6}}
$$
